steel/Zeta.Steel.ExternalPtr.fsti
@@ -14,40 +14,41 @@ val extern_ptr : Type0
 [@@erasable]
 noeq
 type state =
-| Unknown: (in_contents: Seq.seq U8.t) -> state
-| Unread: (in_contents: Seq.seq U8.t) -> (out_len: U32.t) -> state
-| Read: (in_contents: Seq.seq U8.t) -> (out_len: U32.t) -> state
-| Written: (in_len: nat) -> (written: Seq.seq U8.t) -> state
+| Unread: (out_len: U32.t) -> state
+| Read: (out_len: U32.t) -> state
+| Written: (written: Seq.seq U8.t) -> state
 
-let get_in_contents
-  (s: state)
-: Ghost (Seq.seq U8.t)
-    (requires (~ (Written? s)))
-    (ensures (fun _ -> True))
-= match s with
-  | Unknown in_contents
-  | Unread in_contents _
-  | Read in_contents _
-    -> in_contents
+val extern_in_out_pts_to (e1: extern_ptr) (e2: extern_ptr) (in_contents: Seq.seq U8.t) (s: state) : vprop
 
-val extern_in_out_pts_to (e1: extern_ptr) (e2: extern_ptr) (s: state) : vprop
-
-let is_valid_state (b: bool) (in_contents: Seq.seq U8.t) (out_len: U32.t) : Tot state =
-  if b then Unread in_contents out_len else Unknown in_contents
-
-val extern_in_out_pts_to_is_valid
+[@@__reduce__]
+let is_valid_state_true
   (e1: extern_ptr)
-  (w1: Ghost.erased (Seq.seq U8.t))
   (n1: U32.t)
   (e2: extern_ptr)
   (n2: U32.t)
-: ST bool
-  (extern_in_out_pts_to e1 e2 (Unknown w1))
-  (fun b -> extern_in_out_pts_to e1 e2 (is_valid_state b w1 n2))
-  True
-  (fun b -> b == true ==> (
-    U32.v n1 == Seq.length w1
-  ))
+: Tot vprop
+= exists_ (fun in_contents ->
+    extern_in_out_pts_to e1 e2 in_contents (Unread n2) `star`
+    pure (U32.v n1 == Seq.length in_contents)
+  )
+
+let is_valid_state
+  (e1: extern_ptr)
+  (n1: U32.t)
+  (e2: extern_ptr)
+  (n2: U32.t)
+  (b: bool)
+: Tot vprop
+= if b then is_valid_state_true e1 n1 e2 n2 else emp
+
+val extern_in_out_pts_to_is_valid
+  (e1: extern_ptr)
+  (n1: U32.t)
+  (e2: extern_ptr)
+  (n2: U32.t)
+: STT bool
+  emp
+  (fun b -> is_valid_state e1 n1 e2 n2 b)
 
 inline_for_extraction
 val copy_extern_input_ptr
@@ -58,9 +59,9 @@ val copy_extern_input_ptr
   (out_len: Ghost.erased U32.t)
   (a: A.array U8.t)
 : ST unit
-    (extern_in_out_pts_to e1 e2 (Unread w1 out_len) `star` exists_ (fun contents -> A.pts_to a full_perm contents))
+    (extern_in_out_pts_to e1 e2 w1 (Unread out_len) `star` exists_ (fun contents -> A.pts_to a full_perm contents))
     (fun _ ->
-      extern_in_out_pts_to e1 e2 (Read w1 out_len) `star` A.pts_to a full_perm w1
+      extern_in_out_pts_to e1 e2 w1 (Read out_len) `star` A.pts_to a full_perm w1
     )
     (A.length a == U32.v n /\
       Seq.length w1 == U32.v n)
@@ -71,16 +72,14 @@ val copy_extern_output_ptr
   (e1: extern_ptr)
   (w1: Ghost.erased (Seq.seq U8.t))
   (e2: extern_ptr)
-  (in_len: Ghost.erased nat)
   (n: U32.t)
   (a: A.array U8.t)
   (p: perm)
   (contents: Ghost.erased (Seq.seq U8.t))
 : ST unit
-    (extern_in_out_pts_to e1 e2 (Read w1 n) `star` A.pts_to a p contents)
+    (extern_in_out_pts_to e1 e2 w1 (Read n) `star` A.pts_to a p contents)
     (fun _ ->
-      extern_in_out_pts_to e1 e2 (Written in_len contents) `star` A.pts_to a p contents
+      extern_in_out_pts_to e1 e2 w1 (Written contents) `star` A.pts_to a p contents
     )
-    (A.length a == U32.v n /\
-      Seq.length w1 == Ghost.reveal in_len)
+    (A.length a == U32.v n)
     (fun _ -> True)
